Phi_Semantics/PhiSem_Variable.thy
@@ -47,7 +47,8 @@ subsubsection \<open>Fiction\<close>
 
 fiction_space \<phi>var =
   Var :: \<open>RES.Var.basic_fiction \<Zcomp>\<^sub>\<I> \<F>_pointwise (\<lambda>_. \<F>_it)\<close>
-            (pointwise_fiction_for_partial_mapping_resource RES.Var \<open>(\<lambda>_::varname. UNIV :: VAL option nosep set)\<close>) ..
+            (pointwise_fiction_for_partial_mapping_resource RES.Var \<open>(\<lambda>_::varname. UNIV :: VAL option nosep set)\<close>)
+  by (standard; simp add: set_eq_iff fun_eq_iff)
 
 hide_fact FIC.\<phi>var_fic_ax FIC.\<phi>var_fic_axioms
 
